more (code generation works again)

Weidenbach_Book/IsaSAT_CDCL.thy
@@ -35,7 +35,7 @@ definition (in isasat_input_ops) vmtf_find_next_undef_upd
         (((nat, nat)ann_lits \<times> vmtf_remove_int) \<times> nat option)nres\<close>
 where
   \<open>vmtf_find_next_undef_upd = (\<lambda>M vm. do{
-      L \<leftarrow>  vmtf_find_next_undef vm M;
+      L \<leftarrow> vmtf_find_next_undef vm M;
       RETURN ((M, update_next_search L vm), L)
   })\<close>
 
@@ -67,7 +67,7 @@ lemmas vmtf_find_next_undef_upd_code_ref[sepref_fr_rules] =
    vmtf_find_next_undef_upd_code.refine[OF isasat_input_bounded_nempty_axioms]
 
 
-definition lit_of_found_atm where
+definition (in isasat_input_ops)lit_of_found_atm where
 \<open>lit_of_found_atm \<phi> L = SPEC (\<lambda>K. (L = None \<longrightarrow> K = None) \<and>
     (L \<noteq> None \<longrightarrow> K \<noteq> None \<and> atm_of (the K) = the L))\<close>
 
@@ -79,10 +79,11 @@ where
      (L \<noteq> None \<longrightarrow> Pos (the L) \<in> snd ` D\<^sub>0 \<and> undefined_atm M (the L)) \<and>
      (L = None \<longrightarrow> (\<forall>K\<in>snd ` D\<^sub>0. defined_lit M K)) \<and> M = M' \<and> vm \<in> vmtf M)\<close>
 
-definition find_unassigned_lit_wl_D_heur
+definition (in isasat_input_ops) find_unassigned_lit_wl_D_heur
   :: \<open>twl_st_wl_heur \<Rightarrow> (twl_st_wl_heur \<times> nat literal option) nres\<close>
 where
   \<open>find_unassigned_lit_wl_D_heur = (\<lambda>(M, N, U, D, WS, Q, vm, \<phi>, clvls). do {
+      ASSERT(vm \<in> vmtf M \<and> phase_saving \<phi>);
       ((M, vm), L) \<leftarrow> find_undefined_atm M vm;
       L \<leftarrow> lit_of_found_atm \<phi> L;
       RETURN ((M, N, U, D, WS, Q, vm, \<phi>, clvls), L)
@@ -91,7 +92,9 @@ where
 lemma find_unassigned_lit_wl_D'_find_unassigned_lit_wl_D:
   \<open>(find_unassigned_lit_wl_D_heur, find_unassigned_lit_wl_D) \<in>
      [\<lambda>S. twl_struct_invs (twl_st_of_wl None S) \<and> literals_are_\<L>\<^sub>i\<^sub>n S \<and> get_conflict_wl S = None]\<^sub>f
-    twl_st_heur \<rightarrow> \<langle>twl_st_heur \<times>\<^sub>r \<langle>nat_lit_lit_rel\<rangle>option_rel\<rangle>nres_rel\<close>
+    twl_st_heur \<rightarrow> \<langle>{((T, L), (T', L')). (T, T') \<in> twl_st_heur \<and> L = L' \<and>
+         (L \<noteq> None \<longrightarrow> undefined_lit (get_trail_wl T') (the L) \<and> the L \<in># \<L>\<^sub>a\<^sub>l\<^sub>l) \<and>
+         get_conflict_wl T' = None}\<rangle>nres_rel\<close>
 proof -
   have [simp]: \<open>undefined_lit M (Pos (atm_of y)) = undefined_lit M y\<close> for M y
     by (auto simp: defined_lit_map)
@@ -119,6 +122,9 @@ proof -
           mset_take_mset_drop_mset mset_take_mset_drop_mset'
           clauses_def simp del: entailed_clss_inv.simps)
   qed
+  have [dest]: \<open>(S, T) \<in> twl_st_heur \<Longrightarrow> \<phi> = get_phase_saver_heur S \<Longrightarrow> phase_saving \<phi>\<close> for S T \<phi>
+    by (auto simp: twl_st_heur_def)
+    
   show ?thesis
    unfolding find_unassigned_lit_wl_D_heur_def find_unassigned_lit_wl_D_def find_undefined_atm_def
     ID_R lit_of_found_atm_def
@@ -126,7 +132,7 @@ proof -
    apply clarify
    apply refine_vcg
    unfolding RETURN_RES_refine_iff
-   by (fastforce simp add: twl_st_heur_def atms in_\<L>\<^sub>a\<^sub>l\<^sub>l_atm_of_in_atms_of_iff Ball_def image_image
+   by (auto simp add: twl_st_heur_def atms in_\<L>\<^sub>a\<^sub>l\<^sub>l_atm_of_in_atms_of_iff Ball_def image_image
        mset_take_mset_drop_mset'
         simp del: twl_st_of_wl.simps dest!: atms)
 qed
@@ -214,8 +220,7 @@ lemma find_unassigned_lit_wl_D_code_helper:
 sepref_register find_undefined_atm
 sepref_thm find_unassigned_lit_wl_D_code
   is \<open>PR_CONST find_unassigned_lit_wl_D_heur\<close>
-  :: \<open>[\<lambda>(M, N, U, D, WS, Q, vm, \<phi>, clvls). vm \<in> vmtf M \<and> phase_saving \<phi>]\<^sub>a
-     twl_st_heur_assn\<^sup>d \<rightarrow> (twl_st_heur_assn *a option_assn unat_lit_assn)\<close>
+  :: \<open>twl_st_heur_assn\<^sup>d \<rightarrow>\<^sub>a (twl_st_heur_assn *a option_assn unat_lit_assn)\<close>
   supply [[goals_limit=1]] find_unassigned_lit_wl_D_code_helper[simp]
   unfolding find_unassigned_lit_wl_D_heur_def twl_st_heur_assn_def PR_CONST_def
   by sepref
@@ -229,61 +234,9 @@ prepare_code_thms (in -) find_unassigned_lit_wl_D_code_def
 lemmas find_unassigned_lit_wl_D_heur_hnr[sepref_fr_rules] =
    find_unassigned_lit_wl_D_code.refine[of \<A>\<^sub>i\<^sub>n, OF isasat_input_bounded_nempty_axioms]
 
-definition find_unassigned_lit_wl_D_pre where
-  \<open>find_unassigned_lit_wl_D_pre = (\<lambda>S. twl_struct_invs (twl_st_of_wl None S) \<and> literals_are_\<L>\<^sub>i\<^sub>n S \<and>
-             get_conflict_wl S = None)\<close>
-
-lemma find_unassigned_lit_wl_D_hnr[sepref_fr_rules]:
-  \<open>(find_unassigned_lit_wl_D_code, PR_CONST find_unassigned_lit_wl_D)
-  \<in> [find_unassigned_lit_wl_D_pre]\<^sub>a
-    twl_st_assn\<^sup>d \<rightarrow> twl_st_assn *a option_assn unat_lit_assn\<close>
-    (is \<open>?c \<in> [?pre]\<^sub>a ?im \<rightarrow> ?f\<close>)
-proof -
-  have H: \<open>?c
-  \<in> [comp_PRE twl_st_heur
-       (\<lambda>S. twl_struct_invs (twl_st_of_wl None S) \<and>
-             literals_are_\<L>\<^sub>i\<^sub>n S \<and>
-             get_conflict_wl S = None)
-       (\<lambda>_ (M, N, U, D, WS, Q, vm, \<phi>, clvls).
-           vm \<in> vmtf M \<and> phase_saving \<phi>)
-       (\<lambda>_. True)]\<^sub>a hrp_comp (twl_st_heur_assn\<^sup>d)
-                       twl_st_heur \<rightarrow> hr_comp
-         (twl_st_heur_assn *a option_assn unat_lit_assn)
-         (twl_st_heur \<times>\<^sub>f \<langle>nat_lit_lit_rel\<rangle>option_rel)\<close>
-    (is \<open>_ \<in> [?pre']\<^sub>a ?im' \<rightarrow> ?f'\<close>)
-    using hfref_compI_PRE_aux[OF find_unassigned_lit_wl_D_heur_hnr[unfolded PR_CONST_def]
-        find_unassigned_lit_wl_D'_find_unassigned_lit_wl_D[unfolded PR_CONST_def]]
-    unfolding PR_CONST_def
-    .
-  have pre: \<open>?pre x \<Longrightarrow> ?pre' x\<close> for x
-    unfolding comp_PRE_def find_unassigned_lit_wl_D_pre_def
-      by (auto simp: comp_PRE_def twl_st_assn_def twl_st_heur_def
-          map_fun_rel_def intro!: ext)
-  have im: \<open>?im' = ?im\<close>
-    unfolding prod_hrp_comp hrp_comp_dest hrp_comp_keep twl_st_assn_def[symmetric]
-    by (auto simp: hrp_comp_def hr_comp_def)
-  have f: \<open>?f' = ?f\<close>
-    unfolding prod_hrp_comp hrp_comp_dest hrp_comp_keep twl_st_assn_def
-    by (auto simp: hrp_comp_def hr_comp_def)
-  show ?thesis
-    apply (rule hfref_weaken_pre[OF ])
-     defer
-    using H unfolding im f apply assumption
-    using pre ..
-qed
-
-lemma decide_wl_or_skip_D_helper:
-  assumes
-    \<open>decide_wl_or_skip_D_pre (a, aa, ab, ac, ad, ae, af, b)\<close>
-  shows \<open>find_unassigned_lit_wl_D_pre (a, aa, ab, ac, ad, ae, af, b)\<close> and
-     \<open>get_conflict_wl (a, aa, ab, ac, ad, ae, af, b) = None\<close>
-  using assms unfolding decide_wl_or_skip_D_pre_def find_unassigned_lit_wl_D_pre_def
-  decide_wl_or_skip_pre_def decide_l_or_skip_pre_def
-  by auto
-
-definition decide_lit_wl_heur :: \<open>nat literal \<Rightarrow> twl_st_wl_heur \<Rightarrow> twl_st_wl_heur\<close> where
-  \<open>decide_lit_wl_heur = (\<lambda>L' (M, N, U, D, Q, W, vmtf, \<phi>, clvls, cach, lbd, stats).
-      (Decided L' # M, N, U, D, {#- L'#}, W, vmtf, \<phi>, clvls, cach, lbd, incr_decision stats))\<close>
+definition (in isasat_input_ops) decide_lit_wl_heur :: \<open>nat literal \<Rightarrow> twl_st_wl_heur \<Rightarrow> twl_st_wl_heur\<close> where
+  \<open>decide_lit_wl_heur = (\<lambda>L' (M, N, U, D, Q, W, vmtf, \<phi>, clvls, cach, lbd, outl, stats).
+      (Decided L' # M, N, U, D, {#- L'#}, W, vmtf, \<phi>, clvls, cach, lbd, outl, incr_decision stats))\<close>
 
 lemma decide_lit_wl_heur_decide_lit_wl:
   \<open>(uncurry (RETURN oo decide_lit_wl_heur), uncurry (RETURN oo decide_lit_wl)) \<in>
@@ -293,10 +246,10 @@ lemma decide_lit_wl_heur_decide_lit_wl:
   by (intro frefI nres_relI)
     (auto simp: twl_st_heur_def intro: vmtf_consD)
 
-
 sepref_thm decide_lit_wl_code
-  is \<open>uncurry (RETURN oo (PR_CONST decide_lit_wl_heur))\<close>
-  :: \<open>[\<lambda>(L, (M, N, U, D, WS, Q, vm, \<phi>)). undefined_lit M L \<and> L \<in> snd ` D\<^sub>0]\<^sub>a
+  is \<open>uncurry (RETURN oo decide_lit_wl_heur)\<close>
+  :: \<open>[\<lambda>(L, S). undefined_lit (get_trail_wl_heur S) L \<and> get_conflict_wl_heur S = None \<and>
+        L \<in> snd ` D\<^sub>0]\<^sub>a
      unat_lit_assn\<^sup>k *\<^sub>a twl_st_heur_assn\<^sup>d \<rightarrow> twl_st_heur_assn\<close>
   supply [[goals_limit=1]] find_unassigned_lit_wl_D_code_helper[simp]
   unfolding decide_lit_wl_heur_def twl_st_heur_assn_def PR_CONST_def
@@ -313,72 +266,110 @@ prepare_code_thms (in -) decide_lit_wl_code_def
 lemmas decide_lit_wl_heur_hnr[sepref_fr_rules] =
   decide_lit_wl_code.refine[OF isasat_input_bounded_nempty_axioms]
 
-lemma decide_lit_wl_hnr[sepref_fr_rules]:
-  \<open>(uncurry decide_lit_wl_code, uncurry (RETURN \<circ>\<circ> decide_lit_wl))
-  \<in> [\<lambda>(L, S). undefined_lit (get_trail_wl S) L  \<and> L \<in> snd ` D\<^sub>0 \<and>
-      get_conflict_wl S = None]\<^sub>a unat_lit_assn\<^sup>k *\<^sub>a twl_st_assn\<^sup>d \<rightarrow>  twl_st_assn\<close>
-    (is \<open>?c \<in> [?pre]\<^sub>a ?im \<rightarrow> ?f\<close>)
-proof -
-  have H: \<open>?c
-  \<in> [comp_PRE (nat_lit_lit_rel \<times>\<^sub>f twl_st_heur)
-       (\<lambda>(L, S). undefined_lit (get_trail_wl S) L \<and>
-           get_conflict_wl S = None)
-       (\<lambda>_ (L, M, N, U, D, WS, Q, vm, \<phi>).
-           undefined_lit M L \<and> L \<in> snd ` D\<^sub>0)
-       (\<lambda>_. True)]\<^sub>a hrp_comp
-                       (unat_lit_assn\<^sup>k *\<^sub>a
-                        twl_st_heur_assn\<^sup>d)
-                       (nat_lit_lit_rel \<times>\<^sub>f
-                        twl_st_heur) \<rightarrow> hr_comp
-           twl_st_heur_assn twl_st_heur\<close>
-    (is \<open>_ \<in> [?pre']\<^sub>a ?im' \<rightarrow> ?f'\<close>)
-    using hfref_compI_PRE_aux[OF decide_lit_wl_heur_hnr[unfolded PR_CONST_def]
-        decide_lit_wl_heur_decide_lit_wl] .
-  have pre: \<open>?pre x \<Longrightarrow> ?pre' x\<close> for x
-    by (auto simp: comp_PRE_def twl_st_heur_def image_image intro!: ext)
-  have im: \<open>?im' = ?im\<close>
-    unfolding prod_hrp_comp hrp_comp_dest hrp_comp_keep twl_st_assn_def
-    by (auto simp: hrp_comp_def hr_comp_def)
-  have f: \<open>?f' = ?f\<close>
-    unfolding prod_hrp_comp hrp_comp_dest hrp_comp_keep twl_st_assn_def
-    by (auto simp: hrp_comp_def hr_comp_def)
-  show ?thesis
-    apply (rule hfref_weaken_pre[OF ])
-     defer
-    using H unfolding im f apply assumption
-    using pre ..
-qed
+definition(in isasat_input_ops)  decide_wl_or_skip_D_heur
+  :: \<open>twl_st_wl_heur \<Rightarrow> (bool \<times> twl_st_wl_heur) nres\<close>
+where
+  \<open>decide_wl_or_skip_D_heur S = (do {
+    (S, L) \<leftarrow> find_unassigned_lit_wl_D_heur S;
+    case L of
+      None \<Rightarrow> RETURN (True, S)
+    | Some L \<Rightarrow>
+       do {ASSERT(undefined_lit (get_trail_wl_heur S) L \<and> get_conflict_wl_heur S = None \<and>
+             L \<in> snd ` D\<^sub>0); 
+         RETURN (False, decide_lit_wl_heur L S) }
+  })
+\<close>
 
-sepref_register decide_wl_or_skip_D find_unassigned_lit_wl_D
+lemma decide_wl_or_skip_D_heur_decide_wl_or_skip_D:
+  \<open>(decide_wl_or_skip_D_heur, decide_wl_or_skip_D) \<in> twl_st_heur \<rightarrow>\<^sub>f \<langle>bool_rel \<times>\<^sub>f twl_st_heur\<rangle> nres_rel\<close>
+  supply [[goals_limit=1]]
+  unfolding decide_wl_or_skip_D_heur_def decide_wl_or_skip_D_def decide_wl_or_skip_D_pre_def
+  decide_wl_or_skip_pre_def decide_l_or_skip_pre_def twl_st_of_wl.simps[symmetric]
+  apply (intro nres_relI frefI)
+  apply (refine_vcg find_unassigned_lit_wl_D'_find_unassigned_lit_wl_D[THEN fref_to_Down])
+  subgoal by (auto simp del: twl_st_of.simps simp: twl_st_heur_def)
+  subgoal by (auto simp del: twl_st_of.simps simp: twl_st_heur_def)
+  subgoal by (auto simp del: twl_st_of.simps simp: twl_st_heur_def)
+  subgoal by (auto simp del: twl_st_of.simps simp: twl_st_heur_def)
+  subgoal by (auto simp del: twl_st_of.simps simp: twl_st_heur_def)
+  subgoal by (auto simp del: twl_st_of.simps simp: twl_st_heur_def)
+  subgoal by (auto simp del: twl_st_of.simps simp: twl_st_heur_def)
+  subgoal by (auto simp del: twl_st_of.simps)
+  subgoal by (auto simp del: twl_st_of.simps simp: twl_st_heur_def decide_lit_wl_heur_def
+        decide_lit_wl_def counts_maximum_level_def intro!: vmtf_consD)
+  done
+
+sepref_register decide_wl_or_skip_D find_unassigned_lit_wl_D_heur decide_lit_wl_heur
 sepref_thm decide_wl_or_skip_D_code
-  is \<open>PR_CONST decide_wl_or_skip_D\<close>
-  :: \<open>twl_st_assn\<^sup>d \<rightarrow>\<^sub>a bool_assn *a twl_st_assn\<close>
-  unfolding decide_wl_or_skip_D_def PR_CONST_def
-  supply [[goals_limit = 1]] decide_wl_or_skip_D_helper[simp, intro]
+  is \<open>PR_CONST decide_wl_or_skip_D_heur\<close>
+  :: \<open>twl_st_heur_assn\<^sup>d \<rightarrow>\<^sub>a bool_assn *a twl_st_heur_assn\<close>
+  unfolding decide_wl_or_skip_D_heur_def PR_CONST_def
+  supply [[goals_limit = 1]]
     find_unassigned_lit_wl_D_def[simp] image_image[simp]
   by sepref
 
 concrete_definition (in -) decide_wl_or_skip_D_code
-  uses isasat_input_bounded_nempty.decide_wl_or_skip_D_code.refine_raw
-  is \<open>(?f, _) \<in> _\<close>
+   uses isasat_input_bounded_nempty.decide_wl_or_skip_D_code.refine_raw
+   is \<open>(?f,_)\<in>_\<close>
 
 prepare_code_thms (in -) decide_wl_or_skip_D_code_def
 
 lemmas decide_wl_or_skip_D_hnr[sepref_fr_rules] =
-  decide_wl_or_skip_D_code.refine[OF isasat_input_bounded_nempty_axioms]
+   decide_wl_or_skip_D_code.refine[of \<A>\<^sub>i\<^sub>n, OF isasat_input_bounded_nempty_axioms]
+
 
 
 paragraph \<open>Combining Together: the Other Rules\<close>
 
-sepref_register get_conflict_wl_is_None
+definition (in isasat_input_ops) cdcl_twl_o_prog_wl_D_heur
+ :: \<open>twl_st_wl_heur \<Rightarrow> (bool \<times> twl_st_wl_heur) nres\<close>
+where
+  \<open>cdcl_twl_o_prog_wl_D_heur S =
+    do {
+      if get_conflict_wl_heur S = None
+      then decide_wl_or_skip_D_heur S
+      else do {
+        T \<leftarrow> skip_and_resolve_loop_wl_D_heur S;
+        if get_conflict_wl_heur T \<noteq> Some {#}
+        then do {U \<leftarrow> backtrack_wl_D_nlit_heur T; RETURN (False, U)}
+        else do {RETURN (True, T)}
+      }
+    }
+  \<close>
+
+sepref_register get_conflict_wl_is_None decide_wl_or_skip_D_heur skip_and_resolve_loop_wl_D_heur
+  backtrack_wl_D_nlit_heur
+
+(* TODO Move + kill get_conflict_wl_is_Nil *)
+definition (in -)get_conflict_wl_heur_is_Nil :: \<open>twl_st_wl_heur \<Rightarrow> bool\<close> where
+  \<open>get_conflict_wl_heur_is_Nil = (\<lambda>(M, N, U, D, NE, UE, Q, W). D \<noteq> None \<and> Multiset.is_empty (the D))\<close>
+
+lemma get_conflict_wl_heur_is_Nil_alt_def:
+  \<open>get_conflict_wl_heur_is_Nil S \<longleftrightarrow> get_conflict_wl_heur S = Some {#}\<close>
+  by (cases S) (auto simp: get_conflict_wl_heur_is_Nil_def Multiset.is_empty_def)
+
+lemma get_conflict_wl_heur_is_Nil_get_conflict_wll_is_Nil_heur:
+  \<open>RETURN o get_conflict_wl_heur_is_Nil = get_conflict_wll_is_Nil_heur\<close>
+  by (auto intro!: ext simp: get_conflict_wl_heur_is_Nil_def get_conflict_wll_is_Nil_heur_def
+      split: if_splits option.splits)
+
+lemma [sepref_fr_rules]: \<open>(get_conflict_wll_is_Nil_code, RETURN \<circ> get_conflict_wl_heur_is_Nil)
+\<in> twl_st_heur_assn\<^sup>k \<rightarrow>\<^sub>a bool_assn\<close>
+  using get_conflict_wll_is_Nil_code[unfolded PR_CONST_def 
+    get_conflict_wl_heur_is_Nil_get_conflict_wll_is_Nil_heur[symmetric]]
+  .
+
+(* End Move *)
 
 sepref_register cdcl_twl_o_prog_wl_D
+
 sepref_thm cdcl_twl_o_prog_wl_D_code
-  is \<open>PR_CONST cdcl_twl_o_prog_wl_D\<close>
-  :: \<open>twl_st_assn\<^sup>d \<rightarrow>\<^sub>a bool_assn *a twl_st_assn\<close>
-  unfolding cdcl_twl_o_prog_wl_D_def PR_CONST_def
+  is \<open>PR_CONST cdcl_twl_o_prog_wl_D_heur\<close>
+  :: \<open>twl_st_heur_assn\<^sup>d \<rightarrow>\<^sub>a bool_assn *a twl_st_heur_assn\<close>
+  unfolding cdcl_twl_o_prog_wl_D_heur_def PR_CONST_def
   unfolding get_conflict_wl_is_None get_conflict_wl_get_conflict_wl_is_Nil
-    get_conflict_wl_is_None_def[symmetric]
+    get_conflict_wl_is_None_heur_alt_def[symmetric]
+   get_conflict_wl_heur_is_Nil_alt_def[symmetric]
   supply [[goals_limit = 1]]
   by sepref
 
@@ -391,14 +382,46 @@ prepare_code_thms (in -) cdcl_twl_o_prog_wl_D_code_def
 lemmas cdcl_twl_o_prog_wl_D_code[sepref_fr_rules] =
    cdcl_twl_o_prog_wl_D_code.refine[of \<A>\<^sub>i\<^sub>n, OF isasat_input_bounded_nempty_axioms]
 
+lemma
+  \<open>(cdcl_twl_o_prog_wl_D_heur, cdcl_twl_o_prog_wl_D) \<in> twl_st_heur \<rightarrow>\<^sub>f \<langle>bool_rel \<times>\<^sub>f twl_st_heur\<rangle>nres_rel\<close>
+  unfolding cdcl_twl_o_prog_wl_D_heur_def cdcl_twl_o_prog_wl_D_def
+  apply (intro frefI nres_relI)
+  apply (refine_vcg)
+  sorry
 
 paragraph \<open>Combining Together: Full Strategy\<close>
 
-sepref_register cdcl_twl_stgy_prog_wl_D
-sepref_thm cdcl_twl_stgy_prog_wl_D_code
-  is \<open>PR_CONST cdcl_twl_stgy_prog_wl_D\<close>
-  :: \<open>twl_st_assn\<^sup>d \<rightarrow>\<^sub>a twl_st_assn\<close>
-  unfolding cdcl_twl_stgy_prog_wl_D_def PR_CONST_def
+definition (in isasat_input_ops) cdcl_twl_stgy_prog_wl_D_heur
+   :: \<open>twl_st_wl_heur \<Rightarrow> twl_st_wl_heur nres\<close>
+where
+  \<open>cdcl_twl_stgy_prog_wl_D_heur S\<^sub>0 =
+  do {
+    do {
+      (brk, T) \<leftarrow> WHILE\<^sub>T
+        (\<lambda>(brk, _). \<not>brk)
+        (\<lambda>(brk, S).
+        do {
+          T \<leftarrow> unit_propagation_outer_loop_wl_D_heur S;
+          cdcl_twl_o_prog_wl_D_heur T
+        })
+        (False, S\<^sub>0);
+      RETURN T
+    }
+  }
+  \<close>
+
+
+lemma
+  \<open>(cdcl_twl_stgy_prog_wl_D_heur, cdcl_twl_stgy_prog_wl_D) \<in> twl_st_heur \<rightarrow>\<^sub>f \<langle>twl_st_heur\<rangle>nres_rel\<close>
+  sorry
+
+sepref_register cdcl_twl_stgy_prog_wl_D unit_propagation_outer_loop_wl_D_heur
+  cdcl_twl_o_prog_wl_D_heur
+
+sepref_thm cdcl_twl_stgy_prog_wl_D_code 
+  is \<open>PR_CONST cdcl_twl_stgy_prog_wl_D_heur\<close>
+  :: \<open>twl_st_heur_assn\<^sup>d \<rightarrow>\<^sub>a twl_st_heur_assn\<close>
+  unfolding cdcl_twl_stgy_prog_wl_D_heur_def PR_CONST_def
   supply [[goals_limit = 1]]
   by sepref
 
